
\documentclass{article}
%%%%%%%%%%%%%%%%%%%%%%%%%%%%%%%%%%%%%%%%%%%%%%%%%%%%%%%%%%%%%%%%%%%%%%%%%%%%%%%%%%%%%%%%%%%%%%%%%%%%%%%%%%%%%%%%%%%%%%%%%%%%%%%%%%%%%%%%%%%%%%%%%%%%%%%%%%%%%%%%%%%%%%%%%%%%%%%%%%%%%%%%%%%%%%%%%%%%%%%%%%%%%%%%%%%%%%%%%%%%%%%%%%%%%%%%%%%%%%%%%%%%%%%%%%%%
%TCIDATA{OutputFilter=LATEX.DLL}
%TCIDATA{Version=5.50.0.2960}
%TCIDATA{<META NAME="SaveForMode" CONTENT="1">}
%TCIDATA{BibliographyScheme=Manual}
%TCIDATA{Created=Friday, September 27, 2024 10:56:36}
%TCIDATA{LastRevised=Friday, September 27, 2024 11:06:28}
%TCIDATA{<META NAME="GraphicsSave" CONTENT="32">}
%TCIDATA{<META NAME="DocumentShell" CONTENT="Scientific Notebook\Blank Document">}
%TCIDATA{CSTFile=Math with theorems suppressed.cst}
%TCIDATA{PageSetup=72,72,72,72,0}
%TCIDATA{AllPages=
%F=36,\PARA{038<p type="texpara" tag="Body Text" >\hfill \thepage}
%}


\newtheorem{theorem}{Theorem}
\newtheorem{acknowledgement}[theorem]{Acknowledgement}
\newtheorem{algorithm}[theorem]{Algorithm}
\newtheorem{axiom}[theorem]{Axiom}
\newtheorem{case}[theorem]{Case}
\newtheorem{claim}[theorem]{Claim}
\newtheorem{conclusion}[theorem]{Conclusion}
\newtheorem{condition}[theorem]{Condition}
\newtheorem{conjecture}[theorem]{Conjecture}
\newtheorem{corollary}[theorem]{Corollary}
\newtheorem{criterion}[theorem]{Criterion}
\newtheorem{definition}[theorem]{Definition}
\newtheorem{example}[theorem]{Example}
\newtheorem{exercise}[theorem]{Exercise}
\newtheorem{lemma}[theorem]{Lemma}
\newtheorem{notation}[theorem]{Notation}
\newtheorem{problem}[theorem]{Problem}
\newtheorem{proposition}[theorem]{Proposition}
\newtheorem{remark}[theorem]{Remark}
\newtheorem{solution}[theorem]{Solution}
\newtheorem{summary}[theorem]{Summary}
\newenvironment{proof}[1][Proof]{\noindent\textbf{#1.} }{\ \rule{0.5em}{0.5em}}
\input{tcilatex}

\begin{document}


We can combine these formulae to make one expression 
\begin{equation}
f_{B}=\frac{v_{sound}\pm v_{d}}{v_{sound}\mp v_{e}}f_{A}
\end{equation}%
\textbf{where we use the top sign for the speed when the mover (detector or
emitter) is going toward the non-mover}.

\begin{center}
\begin{tabular}{|l|l|l|l|}
\hline
& 
\begin{tabular}{l}
Stationary \\ 
Detector%
\end{tabular}
& 
\begin{tabular}{c}
Detector  \\ 
moves toward  \\ 
Emitter%
\end{tabular}
& 
\begin{tabular}{c}
Detector  \\ 
moves away from  \\ 
Emitter%
\end{tabular}
\\ \hline
\begin{tabular}{l}
Stationary \\ 
Emitter%
\end{tabular}
& $f_{B}=f_{A}$ & $f_{B}=\frac{v_{sound}+v_{d}}{v_{sound}}f_{A}$ & $f_{B}=%
\frac{v_{sound}-v_{d}}{v_{sound}}f_{A}$ \\ \hline
\begin{tabular}{c}
Emitter \\ 
moves toward  \\ 
Detector%
\end{tabular}
& $f_{B}=\frac{v_{sound}}{v_{sound}-v_{e}}f_{A}$ & $f_{B}=\frac{%
v_{sound}+v_{d}}{v_{sound}-v_{e}}f_{A}$ & $f_{B}=\frac{v_{sound}-v_{d}}{%
v_{sound}-v_{e}}f_{A}$ \\ \hline
\begin{tabular}{c}
Emitter \\ 
moves away from  \\ 
Detector%
\end{tabular}
& $f_{B}=\frac{v_{sound}}{v_{sound}+v_{e}}f_{A}$ & $f_{B}=\frac{%
v_{sound}+v_{d}}{v_{sound}+v_{e}}f_{A}$ & $f_{B}=\frac{v_{sound}-v_{d}}{%
v_{sound}+v_{e}}f_{A}$ \\ \hline
\end{tabular}
\end{center}

\end{document}
